Peano.v
@@ -1,8 +1,17 @@
 
-Require Import Defs NameProofs Mix Theories Meta.
+(** * The Theory of Peano Arithmetic and its Coq model *)
+
+(** The NatDed development, Pierre Letouzey, 2019.
+    This file is released under the CC0 License, see the LICENSE file *)
+
+Require Import Defs NameProofs Mix Meta Theories PreModels Models.
 Import ListNotations.
 Local Open Scope bool_scope.
 Local Open Scope eqb_scope.
+
+(** The Peano axioms *)
+
+Definition PeanoSign := Finite.to_infinite peano_sign.
 
 Definition Zero := Fun "O" [].
 Definition Succ x := Fun "S" [x].
@@ -26,7 +35,7 @@ Definition ax8 := ∀∀∀ (#1 = #0 -> #2 * #1 = #2 * #0).
 
 Definition ax9 := ∀ (Zero + #0 = #0).
 Definition ax10 := ∀∀ (Succ(#1) + #0 = Succ(#1 + #0)).
-Definition ax11 := ∀ (Zero * #0 = #0).
+Definition ax11 := ∀ (Zero * #0 = Zero).
 Definition ax12 := ∀∀ (Succ(#1) * #0 = (#1 * #0) + #0).
 
 Definition ax13 := ∀∀ (Succ(#1) = Succ(#0) -> #1 = #0).
@@ -36,152 +45,28 @@ Definition axioms_list :=
   [ ax1; ax2; ax3; ax4; ax5; ax6; ax7; ax8;
     ax9; ax10; ax11; ax12; ax13; ax14 ].
 
-Fixpoint nForall n A :=
-  match n with
-  | 0 => A
-  | S n => (∀ (nForall n A))%form
-  end.
-
-Lemma nForall_check sign n A :
- check sign (nForall n A) = check sign A.
-Proof.
- induction n; simpl; auto.
-Qed.
-
-Lemma nForall_fclosed n A :
- FClosed A -> FClosed (nForall n A).
-Proof.
- induction n; simpl; auto.
-Qed.
-
-Lemma nForall_level n A :
- level (nForall n A) = level A - n.
-Proof.
- induction n; cbn; auto with arith.
- rewrite IHn. omega.
-Qed.
-
-(** Change all bound vars [#n] into [h #n], with lifting
-    under quantifiers *)
-
-Fixpoint form_update n (h:term->term) f :=
- match f with
-  | True | False => f
-  | Pred p args => Pred p (List.map (bsubst n (h (BVar n))) args)
-  | Not f => Not (form_update n h f)
-  | Op o f f' => Op o (form_update n h f) (form_update n h f')
-  | Quant q f' => Quant q (form_update (S n) h f')
- end.
-
-Lemma form_update_check sign (h:term->term) :
- (forall n, check sign (h (BVar n)) = true) ->
- forall f n, check sign f = true ->
-             check sign (form_update n h f) = true.
-Proof.
- intros Hh. induction f; cbn; intros n; auto.
- - destruct predsymbs; auto.
-   rewrite !lazy_andb_iff.
-   rewrite map_length. intuition.
-   rewrite forallb_forall in *. intros t Ht.
-   rewrite in_map_iff in Ht. destruct Ht as (t' & <- & IN).
-   apply check_bsubst_term; auto.
- - rewrite !lazy_andb_iff; intuition.
-Qed.
-
-Lemma bsubst_term_fvars' n (u t : term) :
-  Names.Subset (fvars t) (fvars (bsubst n u t)).
-Proof.
- revert t. fix IH 1. destruct t; cbn; auto with set.
- clear f.
- revert l. fix IH' 1. destruct l; cbn; auto with set.
- intro x. NamesF.set_iff. intros [IN|IN].
- - left; now apply IH.
- - right. now apply IH'.
-Qed.
-
-Lemma bsubst_fvars' n u (f:formula) :
-  Names.Subset (fvars f) (fvars (bsubst n u f)).
-Proof.
- revert n; induction f; cbn; intros n; auto with set.
- - apply (bsubst_term_fvars' n u (Fun "" l)).
- - intro x. NamesF.set_iff. intros [IN|IN].
-   left; now apply IHf1.
-   right; now apply IHf2.
-Qed.
-
-Lemma form_update_fvars (h:term->term) :
- (forall n, FClosed (h (BVar n))) ->
- forall f n, Names.Equal (fvars (form_update n h f)) (fvars f).
-Proof.
- intros Hh. induction f; cbn; intros n; auto with set.
- - intro x. rewrite unionmap_map_in, unionmap_in.
-   split.
-   + intros (a & IN & IN'). exists a; split; auto.
-     apply bsubst_term_fvars in IN.
-     rewrite Names.union_spec in IN. destruct IN; auto.
-     now apply Hh in H.
-   + intros (a & IN & IN'). exists a; split; auto.
-     now apply bsubst_term_fvars'.
- - intros x. NamesF.set_iff. now rewrite IHf1, IHf2.
-Qed.
-
-Lemma form_update_closed (h:term->term) :
- (forall n, FClosed (h (BVar n))) ->
- forall f n, FClosed f -> FClosed (form_update n h f).
-Proof.
- intros. red. rewrite form_update_fvars; auto.
-Qed.
-
-Lemma level_bsubst_term' n (u t : term) :
-  level u <= S n -> level (bsubst n u t) <= level t.
-Proof.
- intro Hu. revert t. fix IH 1. destruct t; cbn; auto.
- - case eqbspec; intros; subst; auto.
- - revert l. fix IH' 1. destruct l; cbn; auto.
-   apply Nat.max_le_compat; auto.
-Qed.
-
-Lemma level_bsubst' n u (f:formula) :
-  level u <= S n -> level (bsubst n u f) <= level f.
-Proof.
- revert n. induction f; cbn; intros n Hu; auto with arith.
- - now apply (level_bsubst_term' n u (Fun "" l)).
- - apply Nat.max_le_compat; auto.
- - apply Nat.pred_le_mono; auto with arith.
-Qed.
-
-Lemma form_update_level (h:term->term) :
- (forall n, level (h (BVar n)) <= S n) ->
- forall f n, level (form_update n h f) <= level f.
-Proof.
- intros Hh. induction f; cbn; intros n; auto.
- - apply (level_bsubst_term' n (h (#n)) (Fun "" l)); auto.
- - apply Nat.max_le_compat; auto.
- - apply Nat.pred_le_mono; auto.
-Qed.
-
-(** Beware, bsubst would not be ok below for turning [#0] into [Succ #0]
-    (no lift on substituted term inside quantifiers).
+(** Beware, [bsubst] is ok below for turning [#0] into [Succ #0], but
+    only since it contains now a [lift] of substituted terms inside
+    quantifiers.
     And the unconventional [∀] before [A[0]] is to get the right
     bounded vars (Hack !). *)
 
-Definition induction_schema A :=
-  let n := level A in
+Definition induction_schema A_x :=
+  let A_0 := bsubst 0 Zero A_x in
+  let A_Sx := bsubst 0 (Succ(#0)) A_x in
   nForall
-    (pred n)
-    (∀ (bsubst 0 Zero A) /\ (∀ (A -> form_update 0 Succ A)) -> ∀ A).
+    (Nat.pred (level A_x))
+    (((∀ A_0) /\ (∀ (A_x -> A_Sx))) -> ∀ A_x).
 
 Local Close Scope formula_scope.
-
-Definition peano_sign' := Finite.to_infinite peano_sign.
 
 Definition IsAx A :=
   List.In A axioms_list \/
   exists B, A = induction_schema B /\
-            check peano_sign' B = true /\
+            check PeanoSign B = true /\
             FClosed B.
 
-Lemma WfAx A : IsAx A -> Wf peano_sign' A.
+Lemma WfAx A : IsAx A -> Wf PeanoSign A.
 Proof.
  intros [ IN | (B & -> & HB & HB')].
  - apply Wf_iff.
@@ -189,27 +74,94 @@ Proof.
    simpl in IN. intuition; subst; reflexivity.
  - repeat split; unfold induction_schema; cbn.
    + rewrite nForall_check. cbn.
-     rewrite check_bsubst, HB; auto.
-     rewrite form_update_check; auto.
+     rewrite !check_bsubst, HB; auto.
    + red. rewrite nForall_level. cbn.
      assert (level (bsubst 0 Zero B) <= level B).
      { apply level_bsubst'. auto. }
-     assert (level (form_update 0 Succ B) <= level B).
-     { apply form_update_level. auto. }
+     assert (level (bsubst 0 (Succ(BVar 0)) B) <= level B).
+     { apply level_bsubst'. auto. }
      omega with *.
    + apply nForall_fclosed. red. cbn.
-     rewrite form_update_fvars; auto.
      assert (FClosed (bsubst 0 Zero B)).
      { red. rewrite bsubst_fvars.
        intro x. rewrite Names.union_spec. cbn. red in HB'. intuition. }
+     assert (FClosed (bsubst 0 (Succ(BVar 0)) B)).
+     { red. rewrite bsubst_fvars.
+       intro x. rewrite Names.union_spec. cbn - [Names.union].
+       rewrite Names.union_spec.
+       generalize (HB' x) (@Names.empty_spec x). intuition. }
      unfold FClosed in *. intuition.
 Qed.
 
 End PeanoAx.
 
+Local Open Scope string.
+
 Definition PeanoTheory :=
- {| sign := Finite.to_infinite peano_sign;
+ {| sign := PeanoSign;
     IsAxiom := PeanoAx.IsAx;
     WfAxiom := PeanoAx.WfAx |}.
 
-(** TODO : modele *)
+(** A Coq model of this Peano theory, based on the [nat] type *)
+
+Definition PeanoFuns : modfuns nat :=
+  fun f =>
+  if f =? "O" then Some (existT _ 0 0)
+  else if f =? "S" then Some (existT _ 1 S)
+  else if f =? "+" then Some (existT _ 2 Nat.add)
+  else if f =? "*" then Some (existT _ 2 Nat.mul)
+  else None.
+
+Definition PeanoPreds : modpreds nat :=
+  fun p =>
+  if p =? "=" then Some (existT _ 2 (@Logic.eq nat))
+  else None.
+
+Lemma PeanoFuns_ok s :
+ funsymbs PeanoSign s = get_arity (PeanoFuns s).
+Proof.
+ unfold PeanoSign, peano_sign, PeanoFuns. simpl.
+ unfold eqb, eqb_inst_string.
+ repeat (case string_eqb; auto).
+Qed.
+
+Lemma PeanoPreds_ok s :
+ predsymbs PeanoSign s = get_arity (PeanoPreds s).
+Proof.
+ unfold PeanoSign, peano_sign, PeanoPreds. simpl.
+ unfold eqb, eqb_inst_string.
+ case string_eqb; auto.
+Qed.
+
+Definition PeanoPreModel : PreModel nat PeanoTheory :=
+ {| someone := 0;
+    funs := PeanoFuns;
+    preds := PeanoPreds;
+    funsOk := PeanoFuns_ok;
+    predsOk := PeanoPreds_ok |}.
+
+Lemma PeanoAxOk A :
+  IsAxiom PeanoTheory A ->
+  forall genv, interp_form PeanoPreModel genv [] A.
+Proof.
+ unfold PeanoTheory. simpl.
+ unfold PeanoAx.IsAx.
+ intros [IN|(B & -> & CK & CL)].
+ - compute in IN. intuition; subst; cbn; intros; subst; omega.
+ - intros genv.
+   unfold PeanoAx.induction_schema.
+   apply interp_nforall.
+   intros stk Len. rewrite app_nil_r. cbn.
+   intros (Base,Step).
+   (* The Peano induction emulated by a Coq induction :-) *)
+   induction m.
+   + specialize (Base 0).
+     apply -> interp_form_bsubst_gen in Base; simpl; eauto.
+   + apply Step in IHm.
+     apply -> interp_form_bsubst_gen in IHm; simpl; eauto.
+     now intros [|k].
+Qed.
+
+Definition PeanoModel : Model nat PeanoTheory :=
+ {| pre := PeanoPreModel;
+    AxOk := PeanoAxOk |}.
